Port RISC-V's pregs to the Registerfile representation
This makes all preg accesses typed, so a large number of proofs must be
adjusted. Some other details change as well due to typing; for example,
trying to execute 64-bit instructions in 32-bit mode is an error.

riscV/Asm.v
@@ -70,7 +70,36 @@ Proof. decide equality. apply ireg_eq. Defined.
 
 Lemma freg_eq: forall (x y: freg), {x=y} + {x<>y}.
 Proof. decide equality. Defined.
-  
+
+Definition ireg_index (i: ireg): Z :=
+  2 + 2 * match i with
+  | X1  =>  1 | X2  =>  2 | X3  =>  3 | X4  =>  4 | X5  =>  5
+  | X6  =>  6 | X7  =>  7 | X8  =>  8 | X9  =>  9 | X10 => 10
+  | X11 => 11 | X12 => 12 | X13 => 13 | X14 => 14 | X15 => 15
+  | X16 => 16 | X17 => 17 | X18 => 18 | X19 => 19 | X20 => 20
+  | X21 => 21 | X22 => 22 | X23 => 23 | X24 => 24 | X25 => 25
+  | X26 => 26 | X27 => 27 | X28 => 28 | X29 => 29 | X30 => 30
+  | X31 => 31
+  end.
+
+Definition ireg0_index (i: ireg0): Z :=
+  match i with
+  | X0 => 1
+  | X i => ireg_index i
+  end.
+
+Definition freg_index (f: freg): Z :=
+  66 + 2 * match f with
+  | F0  =>  0 | F1  =>  1 | F2  =>  2 | F3  =>  3
+  | F4  =>  4 | F5  =>  5 | F6  =>  6 | F7  =>  7
+  | F8  =>  8 | F9  =>  9 | F10 => 10 | F11 => 11
+  | F12 => 12 | F13 => 13 | F14 => 14 | F15 => 15
+  | F16 => 16 | F17 => 17 | F18 => 18 | F19 => 19
+  | F20 => 20 | F21 => 21 | F22 => 22 | F23 => 23
+  | F24 => 24 | F25 => 25 | F26 => 26 | F27 => 27
+  | F28 => 28 | F29 => 29 | F30 => 30 | F31 => 31
+  end.
+
 (** We model the following registers of the RISC-V architecture. *)
 
 Inductive preg: Type :=
@@ -84,12 +113,136 @@ Coercion FR: freg >-> preg.
 Lemma preg_eq: forall (x y: preg), {x=y} + {x<>y}.
 Proof. decide equality. apply ireg_eq. apply freg_eq. Defined.
 
-Module PregEq.
-  Definition t  := preg.
-  Definition eq := preg_eq.
-End PregEq.
+Definition preg_index (p: preg): Z :=
+  match p with
+  | IR i => ireg_index i
+  | FR f => freg_index f
+  | PC   => 64 + 64 + 2 + 1
+  end.
 
-Module Pregmap := EMap(PregEq).
+Lemma preg_index_bounds:
+  forall p: preg,
+  match p with
+  | IR _ =>   0 < preg_index p /\ preg_index p <= 64
+  | FR _ =>  65 < preg_index p /\ preg_index p <= 128
+  | _    => 130 < preg_index p
+  end.
+Proof.
+  destruct p; unfold preg_index; try omega.
+  destruct i; unfold ireg_index; omega.
+  destruct f; unfold freg_index; omega.
+Qed.
+
+Module Preg <: REGISTER_MODEL.
+
+  Definition reg := preg.
+  Definition eq_dec := preg_eq.
+
+  Definition type pr :=
+    match pr with
+    | IR _ | PC => if Archi.ptr64 then Tany64 else Tany32
+    | FR _         => Tany64
+    end.
+
+  Definition quantity_of pr :=
+    match pr with
+    | IR _ | PC => if Archi.ptr64 then Q64 else Q32
+    | FR _         => Q64
+    end.
+
+  Definition chunk_of pr :=
+    match pr with
+    | IR _ | PC => if Archi.ptr64 then Many64 else Many32
+    | FR _         => Many64
+    end.
+
+  Lemma type_cases: forall r, type r = Tany32 \/ type r = Tany64.
+  Proof.
+    destruct r; simpl; auto; destruct Archi.ptr64; auto.
+  Qed.
+
+  Definition ofs (r: preg): Z :=
+    preg_index r.
+
+  (* A register's address: The index of its first byte. *)
+  Definition addr (r: preg): Z :=
+    preg_index r * 4.
+
+  (* The address one byte past the end of register [r]. The next nonoverlapping
+     register may start here. *)
+  Definition next_addr (r: preg): Z := addr r + AST.typesize (type r).
+
+  Remark addr_pos: forall p, addr p > 0.
+  Proof.
+    intros. unfold addr. destruct p as [x|x|]; try destruct x; simpl; omega.
+  Qed.
+
+  Lemma addr_compat: forall p, FragBlock.addr (ofs p) = addr p.
+  Proof.
+    reflexivity.
+  Qed.
+
+  Lemma size_compat:
+    forall p,
+    AST.typesize (type p) = FragBlock.quantity_size (quantity_of p).
+  Proof.
+    intros. unfold type, quantity_of.
+    destruct p; auto; destruct Archi.ptr64; auto.
+  Qed.
+
+  Lemma next_addr_compat: forall p, FragBlock.next_addr (ofs p) (quantity_of p) = next_addr p.
+  Proof.
+    unfold next_addr, addr, ofs, FragBlock.next_addr, FragBlock.addr; intros.
+    rewrite size_compat. auto.
+  Qed.
+
+  Lemma quantity_of_compat:
+    forall p,
+    quantity_of p = quantity_of_typ (type p).
+  Proof.
+    destruct p; simpl; auto; destruct Archi.ptr64; auto.
+  Qed.
+
+  Lemma chunk_of_reg_compat:
+    forall p,
+    chunk_of p = chunk_of_quantity (quantity_of p).
+  Proof.
+    destruct p; simpl; auto; destruct Archi.ptr64; auto.
+  Qed.
+
+  Lemma chunk_of_reg_type:
+    forall p,
+    chunk_of p = chunk_of_type (type p).
+  Proof.
+    destruct p; simpl; auto; destruct Archi.ptr64; auto.
+  Qed.
+
+  Lemma diff_outside_interval:
+    forall r s, r <> s -> next_addr r <= addr s \/ next_addr s <= addr r.
+  Proof.
+    intros.
+    unfold next_addr, addr.
+    assert (TS: forall p, AST.typesize (type p) = 4 \/ AST.typesize (type p) = 8).
+    { intro p. destruct (type_cases p) as [T | T]; rewrite T; auto. }
+    generalize (preg_index_bounds r), (preg_index_bounds s); intros RB SB.
+    destruct r eqn:R, s eqn:S;
+      try congruence;
+      try (destruct (TS r), (TS s); subst; omega);
+      simpl AST.typesize.
+    - (* two iregs *)
+      destruct Archi.ptr64; simpl; destruct i, i0; simpl; try omega; congruence.
+    - (* two fregs *)
+      destruct f, f0; simpl; try omega; congruence.
+  Qed.
+
+End Preg.
+
+Lemma pc_type: subtype Tptr (Preg.type PC) = true.
+Proof.
+  unfold Tptr. simpl; destruct Archi.ptr64; auto.
+Qed.
+
+Module Pregmap := Regfile(Preg).
 
 (** Conventional names for stack pointer ([SP]) and return address ([RA]). *)
 
@@ -437,25 +590,27 @@ Definition program := AST.program fundef unit.
   type [Tint] or [Tlong] (in 64 bit mode),
   and float registers to values of type [Tsingle] or [Tfloat]. *)
 
-Definition regset := Pregmap.t val.
+Definition regset := Pregmap.t.
 Definition genv := Genv.t fundef unit.
 
 Definition get0w (rs: regset) (r: ireg0) : val :=
   match r with
   | X0 => Vint Int.zero
-  | X r => rs r
+  | X r => Pregmap.get r rs
   end.
 
 Definition get0l (rs: regset) (r: ireg0) : val :=
   match r with
   | X0 => Vlong Int64.zero
-  | X r => rs r
+  | X r => Pregmap.get r rs
   end.
 
-Notation "a # b" := (a b) (at level 1, only parsing) : asm.
+Notation "a # b" := (Pregmap.get b a) (at level 1, only parsing) : asm.
 Notation "a ## b" := (get0w a b) (at level 1) : asm.
 Notation "a ### b" := (get0l a b) (at level 1) : asm.
 Notation "a # b <- c" := (Pregmap.set b c a) (at level 1, b at next level) : asm.
+
+Definition pregmap_read rs := fun r => Pregmap.get r rs.
 
 Open Scope asm.
 
@@ -464,8 +619,25 @@ Open Scope asm.
 Fixpoint undef_regs (l: list preg) (rs: regset) : regset :=
   match l with
   | nil => rs
-  | r :: l' => undef_regs l' (rs#r <- Vundef)
+  | r :: l' => (undef_regs l' rs)#r <- Vundef
   end.
+
+Lemma undef_regs_other:
+  forall r rl rs, ~In r rl -> (undef_regs rl rs) # r = rs # r.
+Proof.
+  induction rl; simpl; intros. auto. rewrite Pregmap.gso. apply IHrl. intuition. intuition.
+Qed.
+
+Lemma undef_regs_same:
+  forall r rl rs, In r rl -> (undef_regs rl rs) # r = Vundef.
+Proof.
+  induction rl; simpl; intros. tauto.
+  destruct H.
+  - subst a. rewrite Pregmap.gss. destruct (Preg.chunk_of r); auto.
+  - destruct (Preg.eq_dec r a).
+    + subst a. rewrite Pregmap.gss. destruct (Preg.chunk_of r); auto.
+    + rewrite Pregmap.gso; auto.
+Qed.
 
 (** Assigning a register pair *)
 
@@ -543,6 +715,12 @@ Axiom low_high_half:
   forall id ofs,
   Val.offset_ptr (high_half ge id ofs) (low_half ge id ofs) = Genv.symbol_address ge id ofs.
 
+(** The high part fits into one word. *)
+
+Axiom high_half_type:
+  forall id ofs,
+  Val.has_type (high_half ge id ofs) Tany32.
+
 (** The semantics is purely small-step and defined as a function
   from the current state (a register set + a memory state)
   to either [Next rs' m'] where [rs'] and [m'] are the updated register
@@ -579,14 +757,14 @@ Definition eval_offset (ofs: offset) : ptrofs :=
 
 Definition exec_load (chunk: memory_chunk) (rs: regset) (m: mem)
                      (d: preg) (a: ireg) (ofs: offset) :=
-  match Mem.loadv chunk m (Val.offset_ptr (rs a) (eval_offset ofs)) with
+  match Mem.loadv chunk m (Val.offset_ptr (rs#a) (eval_offset ofs)) with
   | None => Stuck
   | Some v => Next (nextinstr (rs#d <- v)) m
   end.
 
 Definition exec_store (chunk: memory_chunk) (rs: regset) (m: mem)
                       (s: preg) (a: ireg) (ofs: offset) :=
-  match Mem.storev chunk m (Val.offset_ptr (rs a) (eval_offset ofs)) (rs s) with
+  match Mem.storev chunk m (Val.offset_ptr (rs#a) (eval_offset ofs)) (rs#s) with
   | None => Stuck
   | Some m' => Next (nextinstr rs) m'
   end.
@@ -930,13 +1108,13 @@ Definition exec_instr (f: function) (i: instruction) (rs: regset) (m: mem) : out
       let sp := (Vptr stk Ptrofs.zero) in
       match Mem.storev Mptr_any m1 (Val.offset_ptr sp pos) rs#SP with
       | None => Stuck
-      | Some m2 => Next (nextinstr (rs #X30 <- (rs SP) #SP <- sp #X31 <- Vundef)) m2
+      | Some m2 => Next (nextinstr (rs #X30 <- (rs#SP) #SP <- sp #X31 <- Vundef)) m2
       end
   | Pfreeframe sz pos =>
       match Mem.loadv Mptr_any m (Val.offset_ptr rs#SP pos) with
       | None => Stuck
       | Some v =>
-          match rs SP with
+          match rs#SP with
           | Vptr stk ofs =>
               match Mem.free m stk 0 sz with
               | None => Stuck
@@ -958,7 +1136,7 @@ Definition exec_instr (f: function) (i: instruction) (rs: regset) (m: mem) : out
   | Ploadsi rd f =>
       Next (nextinstr (rs#X31 <- Vundef #rd <- (Vsingle f))) m
   | Pbtbl r tbl =>
-      match rs r with
+      match rs#r with
       | Vint n =>
           match list_nth_z tbl (Int.unsigned n) with
           | None => Stuck
@@ -1021,12 +1199,41 @@ Definition preg_of (r: mreg) : preg :=
 
 (** Undefine all registers except SP and callee-save registers *)
 
-Definition undef_caller_save_regs (rs: regset) : regset :=
+Definition undef_caller_save_regs_spec (rs: preg -> val) : preg -> val :=
   fun r =>
     if preg_eq r SP
     || In_dec preg_eq r (List.map preg_of (List.filter is_callee_save all_mregs))
     then rs r
     else Vundef.
+
+Definition pregs_destroyed_at_call :=
+  PC :: IR X3 :: IR X4 :: IR X31 :: IR RA
+     :: (map preg_of (filter (fun m => negb (is_callee_save m)) all_mregs)).
+
+Lemma pregs_destroyed_at_call_correct:
+  forall r,
+  preg_eq r SP
+  || In_dec preg_eq r (List.map preg_of (List.filter is_callee_save all_mregs))
+  =
+  negb (In_dec preg_eq r pregs_destroyed_at_call).
+Proof.
+  intros.
+  destruct r as [x|x|]; try destruct x; auto.
+Qed.
+
+Definition undef_caller_save_regs (rs: regset) : regset :=
+  undef_regs pregs_destroyed_at_call rs.
+
+Lemma undef_caller_save_regs_correct:
+  forall rs r,
+  (undef_caller_save_regs rs) # r = undef_caller_save_regs_spec (fun r' => rs # r) r.
+Proof.
+  intros. unfold undef_caller_save_regs, undef_caller_save_regs_spec.
+  rewrite pregs_destroyed_at_call_correct.
+  destruct (In_dec preg_eq r pregs_destroyed_at_call) as [IN | NOTIN].
+  - rewrite undef_regs_same; auto.
+  - rewrite undef_regs_other; auto.
+Qed.
 
 (** Extract the values of the arguments of an external call.
     We exploit the calling conventions from module [Conventions], except that
@@ -1034,7 +1241,7 @@ Definition undef_caller_save_regs (rs: regset) : regset :=
 
 Inductive extcall_arg (rs: regset) (m: mem): loc -> val -> Prop :=
   | extcall_arg_reg: forall r,
-      extcall_arg rs m (R r) (rs (preg_of r))
+      extcall_arg rs m (R r) (rs#(preg_of r))
   | extcall_arg_stack: forall ofs q bofs v,
       bofs = Stacklayout.fe_ofs_arg + 4 * ofs ->
       Mem.loadv (chunk_of_quantity q) m
@@ -1065,17 +1272,17 @@ Inductive state: Type :=
 Inductive step: state -> trace -> state -> Prop :=
   | exec_step_internal:
       forall b ofs f i rs m rs' m',
-      rs PC = Vptr b ofs ->
+      rs#PC = Vptr b ofs ->
       Genv.find_funct_ptr ge b = Some (Internal f) ->
       find_instr (Ptrofs.unsigned ofs) (fn_code f) = Some i ->
       exec_instr f i rs m = Next rs' m' ->
       step (State rs m) E0 (State rs' m')
   | exec_step_builtin:
       forall b ofs f ef args res rs m vargs t vres rs' m',
-      rs PC = Vptr b ofs ->
+      rs#PC = Vptr b ofs ->
       Genv.find_funct_ptr ge b = Some (Internal f) ->
       find_instr (Ptrofs.unsigned ofs) f.(fn_code) = Some (Pbuiltin ef args res) ->
-      eval_builtin_args ge rs (rs SP) m args vargs ->
+      eval_builtin_args ge (fun r => rs#r) (rs#SP) m args vargs ->
       external_call ef ge vargs m t vres m' ->
       rs' = nextinstr
               (set_res res vres
@@ -1084,11 +1291,11 @@ Inductive step: state -> trace -> state -> Prop :=
       step (State rs m) t (State rs' m')
   | exec_step_external:
       forall b ef args res rs m t rs' m',
-      rs PC = Vptr b Ptrofs.zero ->
+      rs#PC = Vptr b Ptrofs.zero ->
       Genv.find_funct_ptr ge b = Some (External ef) ->
       external_call ef ge args m t res m' ->
       extcall_arguments rs m (ef_sig ef) args ->
-      rs' = (set_pair (loc_external_result (ef_sig ef) ) res (undef_caller_save_regs rs))#PC <- (rs RA) ->
+      rs' = (set_pair (loc_external_result (ef_sig ef) ) res (undef_caller_save_regs rs))#PC <- (rs#RA) ->
       step (State rs m) t (State rs' m').
 
 End RELSEM.
@@ -1099,7 +1306,7 @@ Inductive initial_state (p: program): state -> Prop :=
   | initial_state_intro: forall m0,
       let ge := Genv.globalenv p in
       let rs0 :=
-        (Pregmap.init Vundef)
+        Pregmap.init
         # PC <- (Genv.symbol_address ge p.(prog_main) Ptrofs.zero)
         # SP <- Vnullptr
         # RA <- Vnullptr in
@@ -1108,8 +1315,8 @@ Inductive initial_state (p: program): state -> Prop :=
 
 Inductive final_state: state -> int -> Prop :=
   | final_state_intro: forall rs m r,
-      rs PC = Vnullptr ->
-      rs X10 = Vint r ->
+      rs#PC = Vnullptr ->
+      rs#X10 = Vint r ->
       final_state (State rs m) r.
 
 Definition semantics (p: program) :=
